minor refactoring, proved appraisal alt implementations interchangable

src/Appraisal_Defs.v
@@ -1,43 +1,13 @@
-Require Import Term_Defs Term StAM Maps ConcreteEvidence OptMonad.
+Require Import Term_Defs Term StAM Maps ConcreteEvidence OptMonad Auto.
 
 (* Require Import Impl_appraisal (*MonadAM*). *)
 
-Require Import AutoApp.
-
-Require Import StructTactics.
+Require Import AutoApp StructTactics.
 
 Require Import List.
 Import ListNotations.
 
-Require Import Lia.
-
-Fixpoint encodeEv (e:EvidenceC) : EvBits :=
-  match e with
-  | mtc => []
-  | nnc _ bs => [bs]
-  | uuc _ _ _ _ bs e' =>
-    bs :: (encodeEv e')
-  | ggc _ bs e' =>
-    bs :: (encodeEv e')
-  | hhc _ bs _ =>
-    [bs]
-  | ssc e1 e2 =>
-    (encodeEv e1) ++ (encodeEv e2)
-  | ppc e1 e2 =>
-    (encodeEv e1) ++ (encodeEv e2)
-  end.
-
-Definition checkASP (i:ASP_ID) (args:list Arg) (tpl:Plc) (tid:Plc) (bs:BS) : BS.
-Admitted.
-
-Definition checkSigBits (ls:EvBits) (p:Plc) (sig:BS) : BS.
-Admitted.
-
-Definition checkSig (e:EvidenceC) (p:Plc) (sig:BS) : BS :=
-  checkSigBits (encodeEv e) p sig.
-
-Definition checkHash (e:Evidence) (p:Plc) (hash:BS) : BS.
-Admitted.
+Require Import Lia Coq.Program.Tactics.
 
 Definition peel_bs (ls:EvBits) : option (BS * EvBits) :=
   match ls with
@@ -49,8 +19,6 @@ Inductive wf_ec : EvC -> Prop :=
 | wf_ec_c: forall ls et,
     length ls = et_size et ->
     wf_ec (evc ls et).
-
-
 
 Lemma peel_fact': forall e x y H,
     length e = S x ->
@@ -74,25 +42,78 @@ Proof.
   lia.
 Defined.
 
-Lemma firstn_long: forall (e:list BS) x,
-    length e >= x ->
-    length (firstn x e) = x.
-Proof.
-  intros.
-  eapply firstn_length_le.
-  lia.
-Defined.
 
-Lemma skipn_long: forall (e:list BS) x y,
-    length e = x + y ->
-    length (skipn x e) = y.
-Proof.
-  intros.
-  assert (length (skipn x e) = length e - x).
-  { eapply skipn_length. }
-  lia.
-Defined.
+Fixpoint encodeEv (e:EvidenceC) : EvBits :=
+  match e with
+  | mtc => []
+  | nnc _ bs => [bs]
+  | uuc _ _ _ _ bs e' =>
+    bs :: (encodeEv e')
+  | ggc _ bs e' =>
+    bs :: (encodeEv e')
+  | hhc _ bs _ =>
+    [bs]
+  | ssc e1 e2 =>
+    (encodeEv e1) ++ (encodeEv e2)
+  | ppc e1 e2 =>
+    (encodeEv e1) ++ (encodeEv e2)
+  end.
 
+Fixpoint reconstruct_ev' (ls:EvBits) (et:Evidence) : option EvidenceC :=
+  match et with
+  | mt => (* Some mtc *)
+    match ls with
+    | [] => Some mtc
+    | _ => None
+    end 
+  | uu i args tpl tid et' =>
+    '(bs, ls') <- peel_bs ls ;;
+    x <- reconstruct_ev' ls' et' ;;
+    Some (uuc i args tpl tid bs x)
+  | gg p et' =>
+    '(bs, ls') <- peel_bs ls ;;
+    x <- reconstruct_ev' ls' et' ;;
+    Some (ggc p bs x)
+  | hh p et' =>
+    '(bs, ls') <- peel_bs ls ;;
+     match ls' with
+    | [] => Some (hhc p bs et')
+    | _ => None
+    end 
+   
+  | nn i =>
+    '(bs, ls') <- peel_bs ls ;;
+     match ls' with
+    | [] => Some (nnc i bs)
+    | _ => None
+    end 
+    
+  | ss et1 et2 =>
+    e1 <- reconstruct_ev' (firstn (et_size et1) ls) et1 ;;
+    e2 <- reconstruct_ev' (skipn (et_size et1) ls) et2 ;;
+    Some (ssc e1 e2)
+  | pp et1 et2 =>
+    e1 <- reconstruct_ev' (firstn (et_size et1) ls) et1 ;;
+    e2 <- reconstruct_ev' (skipn (et_size et1) ls) et2 ;;
+    Some (ppc e1 e2)  
+  end.
+
+Definition reconstruct_ev (e:EvC) : option EvidenceC :=
+  match e with
+  | evc ls et => reconstruct_ev' ls et
+  end.
+
+Definition checkASP (i:ASP_ID) (args:list Arg) (tpl:Plc) (tid:Plc) (bs:BS) : BS.
+Admitted.
+
+Definition checkSigBits (ls:EvBits) (p:Plc) (sig:BS) : BS.
+Admitted.
+
+Definition checkSig (e:EvidenceC) (p:Plc) (sig:BS) : BS :=
+  checkSigBits (encodeEv e) p sig.
+
+Definition checkHash (e:Evidence) (p:Plc) (hash:BS) : BS.
+Admitted.
 
 Inductive evidenceEvent: Ev -> Prop :=
 | uev: forall n p i args tpl tid, evidenceEvent (umeas n p i args tpl tid).
@@ -123,3 +144,338 @@ Ltac invEvents :=
   match goal with
   | [H: events _ _ _ _  |- _] => invc H
   end.
+
+Lemma inv_recon_mt: forall ls et,
+    reconstruct_ev' ls et = Some mtc ->
+    et = mt.
+Proof.
+  intros.
+  destruct et; repeat ff; try solve_by_inversion.
+Defined.
+
+Lemma inv_recon_nn: forall ls et n n0,
+    reconstruct_ev' ls et = Some (nnc n n0) ->
+    et = nn n.
+Proof.
+  intros.
+  destruct et; repeat ff; try solve_by_inversion.
+Defined.
+
+Lemma inv_recon_uu: forall ls et n l n0 n1 n2 ec,
+    reconstruct_ev' ls et = Some (uuc n l n0 n1 n2 ec) ->
+    (exists et', et = uu n l n0 n1 et').
+Proof.
+  intros.
+  destruct et; repeat ff; try solve_by_inversion.
+  eauto.
+Defined.
+
+Lemma inv_recon_gg: forall ls et n n0 ec,
+    reconstruct_ev' ls et = Some (ggc n n0 ec) ->
+    (exists et', et = gg n et').
+Proof.
+  intros.
+  destruct et; repeat ff; try solve_by_inversion.
+  eauto.
+Defined.
+
+Lemma inv_recon_hh: forall ls et n n0 et',
+    reconstruct_ev' ls et = Some (hhc n n0 et') ->
+    (et = hh n et' ).
+Proof.
+  intros.
+  destruct et; repeat ff; try solve_by_inversion.
+Defined.
+
+Lemma inv_recon_ss: forall ls et ec1 ec2,
+    reconstruct_ev' ls et = Some (ssc ec1 ec2) ->
+    (exists et1 et2, et = ss et1 et2).
+Proof.
+  intros.
+  destruct et; repeat ff; try solve_by_inversion.
+  eauto.
+Defined.
+
+Lemma inv_recon_pp: forall ls et ec1 ec2,
+    reconstruct_ev' ls et = Some (ppc ec1 ec2) ->
+    (exists et1 et2, et = pp et1 et2).
+Proof.
+  intros.
+  destruct et; repeat ff; try solve_by_inversion.
+  eauto.
+Defined.
+
+Lemma firstn_long: forall (e:list BS) x,
+    length e >= x ->
+    length (firstn x e) = x.
+Proof.
+  intros.
+  eapply firstn_length_le.
+  lia.
+Defined.
+
+Lemma skipn_long: forall (e:list BS) x y,
+    length e = x + y ->
+    length (skipn x e) = y.
+Proof.
+  intros.
+  assert (length (skipn x e) = length e - x).
+  { eapply skipn_length. }
+  lia.
+Defined.
+
+Lemma recon_encodeEv : forall ls et ec,
+    wf_ec (evc ls et) -> 
+    reconstruct_ev' ls et = Some ec ->
+    ls = encodeEv ec.
+Proof.
+  intros.
+  generalizeEverythingElse ec.
+  induction ec; intros.
+  -
+    ff.
+    assert (et = mt).
+    {
+      eapply inv_recon_mt; eauto.
+    }
+    subst.
+    invc H.
+    ff.
+    destruct ls; try solve_by_inversion.
+  (* TODO: exclude mt case? *)
+  -
+    ff.
+    assert (et = nn n).
+    {
+      eapply inv_recon_nn; eauto.
+    }
+    subst.
+    repeat ff.
+    destruct ls; try solve_by_inversion.
+
+    (*
+    invc H.
+    ff.
+    assert (e = []).
+    destruct e; try solve_by_inversion.
+    ff. *)
+  -
+    ff.
+    assert (exists et', et = uu n l n0 n1 et').
+    {
+      eapply inv_recon_uu; eauto.
+    }
+    destruct_conjs.
+    subst.
+    repeat ff.
+    invc H.
+    ff.
+    edestruct IHec with (ls := e).
+    2: {
+      eassumption.
+    }
+    econstructor.
+    destruct ls; try solve_by_inversion.
+    unfold peel_bs in *.
+    ff.
+  -
+    ff.
+    assert (exists et', et = gg n et').
+    {
+      eapply inv_recon_gg; eauto.
+    }
+    destruct_conjs.
+    subst.
+    repeat ff.
+    invc H.
+    ff.
+    edestruct IHec with (ls := e).
+    2: {
+      eassumption.
+    }
+    econstructor.
+    destruct ls; try solve_by_inversion.
+    unfold peel_bs in *.
+    ff.
+  -
+    ff.
+    assert (et = hh n e).
+    {
+      eapply inv_recon_hh; eauto.
+    }
+    subst.
+    repeat ff.
+    invc H.
+    ff.
+    destruct ls; try solve_by_inversion.
+  -
+    ff.
+    assert (exists et1 et2, et = ss et1 et2).
+    {
+      eapply inv_recon_ss; eauto.
+    }
+    destruct_conjs.
+    subst.
+    repeat ff.
+    invc H.
+    ff.
+
+    assert ((firstn (et_size H1) ls) = encodeEv ec1).
+    { eapply IHec1 with (et:= H1).
+      econstructor.
+      eapply firstn_long.
+      lia.
+      eassumption.
+    }
+
+    assert ((skipn (et_size H1) ls) = encodeEv ec2).
+    {
+      eapply IHec2 with (et := H2).
+      econstructor.
+      eapply skipn_long.
+      lia.
+      eassumption.
+    }
+    jkjke'.
+    jkjke'.
+    rewrite firstn_skipn.
+    tauto.
+    -
+      ff.
+    assert (exists et1 et2, et = pp et1 et2).
+    {
+      eapply inv_recon_pp; eauto.
+    }
+    destruct_conjs.
+    subst.
+    repeat ff.
+    invc H.
+    ff.
+
+    assert ((firstn (et_size H1) ls) = encodeEv ec1).
+    { eapply IHec1 with (et:= H1).
+      econstructor.
+      eapply firstn_long.
+      lia.
+      eassumption.
+    }
+
+    assert ((skipn (et_size H1) ls) = encodeEv ec2).
+    {
+      eapply IHec2 with (et := H2).
+      econstructor.
+      eapply skipn_long.
+      lia.
+      eassumption.
+    }
+    jkjke'.
+    jkjke'.
+    rewrite firstn_skipn.
+    tauto.
+Defined.
+
+Lemma wf_recon: forall e et ec,
+    reconstruct_ev' e et = Some ec ->
+    wf_ec (evc e et).
+Proof.
+  intros.
+  generalizeEverythingElse ec.
+  induction ec; intros.
+  -
+    assert (et = mt).
+    eapply inv_recon_mt; eauto.
+    subst.
+    repeat ff.
+    econstructor.
+    tauto.
+  -
+    assert (et = nn n) by (eapply inv_recon_nn; eauto).
+    subst.
+    repeat ff.
+    econstructor.
+    ff.
+    destruct e; try solve_by_inversion.
+  -
+    assert (exists et', et = uu n l n0 n1 et').
+    { eapply inv_recon_uu; eauto. }
+    destruct_conjs.
+    subst.
+    repeat ff.
+    assert (wf_ec (evc e0 H0)) by eauto.
+    econstructor.
+    ff.
+    invc H.
+    destruct e; try solve_by_inversion.
+    ff.
+    lia.
+  -
+    assert (exists et', et = gg n et').
+    { eapply inv_recon_gg; eauto. }
+    destruct_conjs.
+    subst.
+    repeat ff.
+    assert (wf_ec (evc e0 H0)) by eauto.
+    econstructor.
+    ff.
+    invc H.
+    destruct e; try solve_by_inversion.
+    ff.
+    lia.
+  -
+    assert (et = hh n e).
+    { eapply inv_recon_hh; eauto.
+    }
+    subst.
+    repeat ff.
+    
+    
+    econstructor.
+    ff.
+    destruct e0; try solve_by_inversion.
+  -
+    assert (exists et1 et2, et = ss et1 et2).
+    { eapply inv_recon_ss; eauto. }
+    destruct_conjs.
+    subst.
+    repeat ff.
+
+    assert (wf_ec (evc (firstn (et_size H0) e) H0)) by eauto.
+
+    assert (wf_ec (evc (skipn (et_size H0) e) H1)) by eauto.
+
+    invc H; invc H2.
+    econstructor.
+    ff.
+    rewrite <- H4.
+    rewrite <- H3.
+    assert (e = (firstn (et_size H0) e) ++ (skipn (et_size H0) e)).
+    
+    { rewrite firstn_skipn.
+      tauto.
+    }
+    rewrite H at 1.
+    eapply app_length.
+  -
+    assert (exists et1 et2, et = pp et1 et2).
+    { eapply inv_recon_pp; eauto. }
+    destruct_conjs.
+    subst.
+    repeat ff.
+
+    assert (wf_ec (evc (firstn (et_size H0) e) H0)) by eauto.
+
+    assert (wf_ec (evc (skipn (et_size H0) e) H1)) by eauto.
+
+    invc H; invc H2.
+    econstructor.
+    ff.
+    rewrite <- H4.
+    rewrite <- H3.
+    assert (e = (firstn (et_size H0) e) ++ (skipn (et_size H0) e)).
+    
+    { rewrite firstn_skipn.
+      tauto.
+    }
+    rewrite H at 1.
+    eapply app_length.
+Defined.
